trans2LTL

LTS.thy
@@ -23,9 +23,8 @@ that @{term "LTS_is_reachable \<Delta>"} is the reflexive, transitive closure of
 
 inductive LTS_is_reachable :: "(('q, 'a) LTS * ('q * 'q) set) \<Rightarrow> 'q \<Rightarrow> 'a list \<Rightarrow> 'q \<Rightarrow> bool" where
    LTS_Empty[intro!]:"LTS_is_reachable lts q [] q"|
-   LTS_Step1[intro!]:"(\<exists>q''. (q, q'') \<in> snd lts \<and> LTS_is_reachable lts q'' l q') \<Longrightarrow> LTS_is_reachable lts q l q'" |
+   LTS_Step1:"(\<exists>q''. (q, q'') \<in> snd lts \<and> LTS_is_reachable lts q'' l q') \<Longrightarrow> LTS_is_reachable lts q l q'" |
    LTS_Step2[intro!]:"(\<exists>q'' \<sigma>. a \<in> \<sigma> \<and> (q, \<sigma>, q'') \<in> fst lts \<and> LTS_is_reachable lts q'' w q') \<Longrightarrow> LTS_is_reachable lts q (a # w) q'"
-
 
 
 
@@ -37,12 +36,25 @@ lemma DeltLTSlemma1:"LTS_is_reachable l q al y \<Longrightarrow>LTS_is_reachable
   next
     case (LTS_Step1 q lts l q')
     then show ?case apply auto
-      by blast
+      by (metis LTS_is_reachable.LTS_Step1 mem_Collect_eq pred_equals_eq2 snd_eqD)
   next
     case (LTS_Step2 a q lts w q')
     then show ?case apply auto by blast
   qed
 
+
+lemma DeltLTSlemma:"LTS_is_reachable l q al y \<Longrightarrow>LTS_is_reachable ({(f u, v, f w)| u v w. (u,v,w)\<in> fst l},{(f u, f w)| u w .(u,w) \<in> snd l}) (f q) al (f y)"
+  proof (induction rule: LTS_is_reachable.induct)  
+    case (LTS_Empty lts q)
+    then show ?case by auto
+  next
+    case (LTS_Step1 q lts l q')
+    then show ?case apply auto
+      by (metis LTS_is_reachable.LTS_Step1 mem_Collect_eq pred_equals_eq2 snd_eqD)
+  next
+    case (LTS_Step2 a q lts w q')
+    then show ?case apply auto by blast
+  qed
 
 
 lemma joinLTSlemma[simp]:"LTS_is_reachable l q x p \<Longrightarrow>  LTS_is_reachable l p y q''\<Longrightarrow> LTS_is_reachable l q (x@y) q''"
@@ -51,7 +63,8 @@ lemma joinLTSlemma[simp]:"LTS_is_reachable l q x p \<Longrightarrow>  LTS_is_rea
     then show ?case apply auto done
   next
     case (LTS_Step1 q lts l q')
-    then show ?case apply auto done
+    then show ?case apply auto 
+      by (meson LTS_is_reachable.LTS_Step1)
   next
     case (LTS_Step2 a q lts w q')
     then show ?case apply auto done
@@ -67,12 +80,14 @@ lemma subLTSlemma[simp]:"LTS_is_reachable l1 q x y \<Longrightarrow> LTS_is_reac
     then show ?case by auto
   next
     case (LTS_Step1 q lts l q')
-    then show ?case by auto
+    then show ?case 
+      by (metis LTS_is_reachable.LTS_Step1 UnI1 snd_conv)
   next
     case (LTS_Step2 a q lts w q')
     then show ?case 
       by (smt (z3) LTS_is_reachable.LTS_Step2 UnI1 fst_conv)
   qed
+
 
 end
 (*
